template-coq/theories/SPropExamples.v
@@ -1,0 +1,15 @@
+Require Import MetaCoq.Template.Ast.
+Require Import MetaCoq.Template.Loader.
+
+Inductive sle : nat -> nat -> SProp :=
+  sle_0 : forall n, sle 0 n
+| sle_S : forall n m : nat, sle n m -> sle (S n) (S m).
+
+Definition blah : sle 0 0 := sle_0 _.
+
+Locate Relevant.
+Locate nAnon.
+
+MetaCoq Quote Recursively Definition zzz' := (fun x : nat => x).
+
+MetaCoq Quote Recursively Definition zzz := blah.
