template-coq/theories/TypingWf.v
@@ -651,6 +651,8 @@ Proof.
            destruct indices_matter; [|trivial].
            eapply type_local_ctx_impl; tea. eauto.
        --- apply (onIndices X1).
+       --- split. apply ind_sorts. destruct indices_matter; auto.
+           eapply type_local_ctx_impl. eapply ind_sorts. auto.
     -- red in onP. red.
        eapply All_local_env_impl. eauto.
        intros. now apply X.
